Tried to implement run semantics. Failed since Coq cannot understand that my recursive function will indeed terminate. If there is an easy way to advance we should learn this, otherwise things will become quite complex.

Relational2.v
@@ -28,10 +28,12 @@ Inductive Exp : Set :=
 Inductive VarName : Set :=
   | ResultName : VarName.
 
+Inductive Statement : Set :=
+  | Assign : VarName -> Exp -> Statement.
+
 Inductive ImpProgram : Set :=
-  | Seq : ImpProgram -> ImpProgram -> ImpProgram
-  | Assign : VarName -> Exp -> ImpProgram
-  | Skip : ImpProgram.
+  | Seq : Statement -> ImpProgram -> ImpProgram
+  | Skip.
 
 Definition queryToImp (q : Query) : option ImpProgram :=
   match q with
@@ -41,33 +43,90 @@ Definition queryToImp (q : Query) : option ImpProgram :=
                  end
   end.
 
-Definition runImp (p : ImpProgram) (r : relation) : option relation :=
- let fix helper (p : ImpProgram) (result : relation) : ImpProgram * relation := 
+Fixpoint runStatement (s: Statement) (input: relation) : option relation :=
+  match s with
+  | Assign vn e => match vn with
+                   | ResultName => match e with
+                                   | InputRelation => Some input
+                                   | RelationExp rexp => Some rexp 
+                                   end
+                   end
+  end.
+
+Fixpoint runImpSmall (p: ImpProgram) (result: option relation) (input: relation) 
+    : ImpProgram  * option relation :=
   match p with
-   | Seq p1 p2 => match p1 with
-                    | Skip => (p2, result) 
-                    | _ => let (p1', result') := helper p1 result in
-                      (Seq p1' p2, result')
-                  end
-   | Assign vn e => match vn with
-                     | ResultName => match e with
-                                       | InputRelation => (Skip, r)
-                                       | RelationExp rexp => (Skip, rexp) 
-                                     end
-                    end
-   | Skip => (Skip, result)
-  end
-  in 
-  let (_, result ) := helper p Rnil in
-    Some result.
+  | Seq s p' => let result' := runStatement s input
+                in (p', result')
+  | Skip => (Skip, None) (* Make this case an exception? *)
+  end.
+
+Definition runImp (p : ImpProgram) (input : relation) : option relation :=
+  let fix helper (p : ImpProgram) (result: option relation) : option relation := 
+    match p with
+      | Skip => result
+      | _ => let (p', result') := runImpSmall p result input
+            in helper p' result'
+    end
+  in helper p (Some Rnil).
+
+(* KM: I did not have a chance to look at below, it is very much chaotic. *)
+
+(*
+Lemma SkipNoop: forall (p: ImpProgram) (r r': relation), 
+   runImp (Seq p Skip) r = Some r' -> runImp p r = Some r'.
+   intros.
+   induction p.
+   
+   compute in IHp1.
+   crush.
+admit.
 
 
+Lemma SkipNoop' : forall (p: ImpProgram) (r r': relation), 
+    runImp p r = Some r' -> runImp (Seq p Skip) r = Some r'.    
+    intros.
+    induction p.
+    
+    .
+*)
 
 Theorem queryEquivalence : forall (q : Query) (p : ImpProgram),
                               queryToImp q = Some p ->
                                  forall (r r' : relation), runQuery q r = Some r' ->
-                                                           runImp p r = Some r'.                intros.
- induction p.
+                                                           runImp p r = Some r'.
+    intros.
+    (*
+    unfold queryToImp in H.
+    destruct q in H.
+    destruct b in H.
+    inversion H.
+    *)
+    induction p.
+
+    
+    unfold queryToImp in H.
+    destruct q in H.
+    destruct b in H.
+    inversion H.
+    unfold runImp.
+    rewrite <- H3 in IHp2. clear H3.
+    rewrite <- H2 in IHp1. clear H2.
+    apply H0.
+    
+    admit.
+    
+    (* program = Assign v e *)
+    unfold queryToImp in H.
+    destruct q in H.
+    destruct b in H.
+    inversion H.
+
+    unfold queryToImp in H.
+    destruct q in H.
+    destruct b in H.
+    inversion H.
+Qed.
  unfold runImp in 
  
  crush.
